src/proofs/ElimLet/BindingProofs.v
@@ -1,0 +1,167 @@
+(*Proofs about [t_open_bound] and similar*)
+Require Import TermFuncs StateHoareMonad StateInvarPres.
+
+Local Open Scope Z_scope.
+
+(*Part 1: Prove things about state modification and invariant preservation (not output)*)
+
+(*Useful in multiple places*)
+Lemma fresh_vsymbol_lt v:
+  st_spec (fun _ : Z => True) (fresh_vsymbol v) (fun (s1 : Z) (_ : TermDefs.vsymbol) (s2 : Z) => s1 < s2).
+Proof.
+  unfold fresh_vsymbol, create_vsymbol.
+  apply prove_st_spec_bnd_invar with (Q1:=fun i j => i < j)(Q2:=fun i j => i <= j); [| | intros; lia].
+  2: { intros x. apply prove_st_spec_ret. intros; lia. }
+  (*Prove [id_register]*)
+  unfold id_register.
+  apply prove_st_spec_bnd_invar with (Q1:=fun i j => i < j)(Q2:=fun i j => i <= j); [| | intros; lia].
+  - (*incr*) apply IdCtr.st_spec_incr. intros.
+    (*TODO: bad*) Transparent CoqBigInt.succ. unfold CoqBigInt.succ. lia. Opaque CoqBigInt.succ.
+  - (*rest of function*) intros _.
+    apply prove_st_spec_bnd_invar with (Q1:=fun i j => i <= j)(Q2:=fun i j => i <= j); [| | intros; lia].
+    + (*get*) apply IdCtr.st_spec_get. intros; lia.
+    + intros x. apply prove_st_spec_ret. intros; lia.
+Qed.
+
+Lemma vs_rename_lt m v:
+  st_spec (fun _ : Z => True) (vs_rename m v)
+  (fun (s1 : Z) (_ : Mvs.t term_c * TermDefs.vsymbol) (s2 : Z) => s1 < s2).
+Proof.
+  unfold vs_rename.
+  apply prove_st_spec_bnd_invar with (Q1:=fun i j => i < j)(Q2:=fun i j => i <= j); [| | intros; lia].
+  2: { intros x. apply prove_st_spec_ret. intros; lia. }
+  (*Prove [fresh_vsymbol]*)
+  apply fresh_vsymbol_lt.
+Qed.
+
+
+(*NOTE: it is important that it increases the state*)
+Lemma t_open_bound_lt b:
+  st_spec (fun _ : Z => True) (t_open_bound b)
+  (fun (s1 : Z) (_ : TermDefs.vsymbol * term_c) (s2 : Z) => (s1 < s2)%Z).
+Proof.
+  unfold t_open_bound.
+  destruct b as [[v ?] t].
+  apply prove_st_spec_bnd_invar with (Q1:=fun i j => i < j)(Q2:=fun i j => i <= j); [| | intros; lia].
+  2: { intros [m t1]. apply prove_st_spec_ret. intros; lia. }
+  (*Prove [vs_rename]*)
+  apply vs_rename_lt.
+Qed.
+
+Lemma t_open_bound_pres tb:
+errst_spec (fun _ : full_st => True) (errst_tup1 (errst_lift1 (t_open_bound tb)))
+  (fun (s1 : full_st) (_ : TermDefs.vsymbol * term_c) (s2 : full_st) => term_wf_pres_cond s1 s2).
+Proof.
+  unfold term_wf_pres_cond.
+  apply errst_spec_tup1 with (P:=fun s1 _ s2 => (s1 <= s2)%Z)(Q:=fun s1 _ s2 =>
+    ((hashcons_ctr (fst (fst (fst s1))) <= hashcons_ctr (fst (fst (fst s2))))%Z /\
+   hashset_subset ty_hash ty_eqb (hashcons_hash (fst (fst (fst s1)))) (hashcons_hash (fst (fst (fst s2)))))).
+  - intros s _. split; try lia. unfold hashset_subset. auto.
+  - (*separate lemma?*)
+    apply errst_spec_st. eapply st_spec_weaken_post. 2: apply t_open_bound_lt.
+    simpl. intros; lia.
+Qed.
+
+(*And for [t_open_branch]*)
+
+(*NOTE: 2 possible specs here: if the pattern has at least one variable, we get <.
+  In all cases, get <=*)
+Lemma t_open_branch_lt b:
+  st_spec (fun _ : Z => True) (t_open_branch b)
+  (fun (s1 : Z) (_ : pattern_c * term_c) (s2 : Z) =>
+    if null (Svs.elements (pat_vars_of (fst (fst b)))) then (s1 <= s2) else (s1 < s2)%Z).
+Proof.
+  unfold t_open_branch.
+  destruct b as [[p ?] t]. simpl.
+  apply prove_st_spec_bnd_invar with 
+  (Q1:=fun i j => if null (Svs.elements (pat_vars_of p)) then i <= j else i < j)
+  (Q2:=fun i j => i <= j).
+  3: { destruct (null (Svs.elements (pat_vars_of p))); auto; intros; lia. }
+  2: { intros [m t1]. apply prove_st_spec_ret. intros; lia. }
+  (*Prove [pat_rename]*)
+  unfold pat_rename.
+  apply prove_st_spec_bnd_invar with 
+  (Q1:=fun i j => if null (Svs.elements (pat_vars_of p)) then i <= j else i < j)
+  (Q2:=fun i j => i <= j).
+  3: { destruct (null (Svs.elements (pat_vars_of p))); auto; intros; lia. }
+  2: { intros [m t1]. apply prove_st_spec_ret. intros; lia. }
+  (*Prove [add_vars]*)
+  induction (Svs.elements (pat_vars_of p)) as [| h tl IH]; simpl; auto.
+  - apply prove_st_spec_ret. intros; lia.
+  - (*bind with [fresh_vsymbol]*)
+    apply prove_st_spec_bnd_invar with (Q1:=fun i j => i < j)(Q2:=fun i j => i <= j); [| | intros; lia].
+    + apply fresh_vsymbol_lt.
+    + intros s1.
+      (*Now either way get <= result*)
+      apply prove_st_spec_bnd_invar with (Q1:=fun i j => i <= j)(Q2:=fun i j => i <= j); [| | intros; lia]; auto.
+      * eapply st_spec_weaken_post. 2: apply IH. simpl. intros. destruct (null tl); lia.
+      * intros. apply prove_st_spec_ret. intros; lia.
+Qed.
+
+Lemma t_open_branch_pres b:
+errst_spec (fun _ : full_st => True) (errst_tup1 (errst_lift1 (t_open_branch b)))
+  (fun (s1 : full_st) (_ : pattern_c * term_c) (s2 : full_st) => term_wf_pres_cond s1 s2).
+Proof.
+  unfold term_wf_pres_cond.
+  apply errst_spec_tup1 with (P:=fun s1 _ s2 => (s1 <= s2)%Z)(Q:=fun s1 _ s2 =>
+    ((hashcons_ctr (fst (fst (fst s1))) <= hashcons_ctr (fst (fst (fst s2))))%Z /\
+   hashset_subset ty_hash ty_eqb (hashcons_hash (fst (fst (fst s1)))) (hashcons_hash (fst (fst (fst s2)))))).
+  - intros s _. split; try lia. unfold hashset_subset. auto.
+  - (*separate lemma?*)
+    apply errst_spec_st. eapply st_spec_weaken_post. 2: apply t_open_branch_lt.
+    simpl. intros; destruct (null _); lia.
+Qed.
+
+(*And [t_open_quant1]*)
+
+Print term_quant.
+Lemma t_open_quant1_lt tq:
+  st_spec (fun _ : Z => True) (t_open_quant1 tq)
+  (fun (s1 : Z) (_ : (list TermDefs.vsymbol * trigger * term_c)) (s2 : Z) => 
+    if null (fst (fst (fst tq))) then s1 <= s2 else (s1 < s2)%Z).
+Proof.
+  unfold t_open_quant1.
+  destruct tq as [[[vs ?] tr] t]. simpl.
+  apply prove_st_spec_bnd_invar with (Q1:=fun i j => if null vs then i <= j else i < j)
+  (Q2:=fun i j => i <= j).
+  3: { destruct (null vs); intros; lia. }
+  2: { intros [m t1]. apply prove_st_spec_ret. intros; lia. }
+  (*Prove [vs_rename]*)
+  unfold vs_rename.
+  apply prove_st_spec_bnd_invar with (Q1:=fun i j => if null vs then i <= j else i < j)
+  (Q2:=fun i j => i <= j).
+  3: { destruct (null vs); intros; lia. }
+  2: { intros x. apply prove_st_spec_ret. intros; lia. }
+  (*[vl_rename_aux*)
+  (*NOTE: this is really annoying to work with*)
+  remember (st_ret (Mvs.empty, [])) as base.
+  assert (Hbase: st_spec (fun _ => True) base (fun s1 _ s2 => s1 <= s2)).
+  { rewrite Heqbase. apply prove_st_spec_ret. intros; lia. }
+  clear Heqbase. generalize dependent base.
+  induction vs as [| h tl IH]; simpl; auto.
+  intros base Hbase.
+  (*bind base*)
+  apply prove_st_spec_bnd_invar with (Q1:=fun i j => i <= j)(Q2:=fun i j => i < j); [| | intros; lia]; auto.
+  intros [m vls]. 
+  (*bind rename*)
+  apply prove_st_spec_bnd_invar with (Q1:=fun i j => i < j)(Q2:=fun i j => i <= j); [| | intros; lia]; auto.
+  + (*vs_rename*) apply vs_rename_lt.
+  + intros [m1 v1]. eapply st_spec_weaken_post. 2: apply IH.
+    * simpl. intros. destruct (null tl); lia.
+    * apply prove_st_spec_ret. intros; lia.
+Qed.
+
+Lemma t_open_quant1_pres tq:
+errst_spec (fun _ : full_st => True) (errst_tup1 (errst_lift1 (t_open_quant1 tq)))
+  (fun (s1 : full_st) (_ : list TermDefs.vsymbol * trigger * term_c) (s2 : full_st) =>
+   term_wf_pres_cond s1 s2).
+Proof.
+  unfold term_wf_pres_cond.
+  apply errst_spec_tup1 with (P:=fun s1 _ s2 => (s1 <= s2)%Z)(Q:=fun s1 _ s2 =>
+    ((hashcons_ctr (fst (fst (fst s1))) <= hashcons_ctr (fst (fst (fst s2))))%Z /\
+   hashset_subset ty_hash ty_eqb (hashcons_hash (fst (fst (fst s1)))) (hashcons_hash (fst (fst (fst s2)))))).
+  - intros s _. split; try lia. unfold hashset_subset. auto.
+  - (*separate lemma?*)
+    apply errst_spec_st. eapply st_spec_weaken_post. 2: apply t_open_quant1_lt.
+    simpl. destruct (null _); intros; lia.
+Qed.
