src/proofs/ElimLet/SubstitutionProofs.v
@@ -1,0 +1,120 @@
+(*Proofs about stateful substitution*)
+Require Export TermTraverse StateInvarPres BindingProofs.
+
+(*part 1: invariant preservation*)
+
+
+(*Useful for these lemmas*)
+Ltac refl_case := intros; apply term_wf_pres_cond_refl.
+Ltac trans_case := intros ? ? ?; apply term_wf_pres_cond_trans.
+
+Lemma t_make_wf_pres t:
+errst_spec (fun _ : full_st => True) (t_make_wf t)
+  (fun (s1 : full_st) (_ : term_c) (s2 : full_st) => term_wf_pres_cond s1 s2).
+Proof.
+ apply tm_traverse_ind with (P:= fun f1 t1 =>
+  errst_spec (fun _ : full_st => True) t1
+    (fun (s1 : full_st) (_ : term_c) (s2 : full_st) => term_wf_pres_cond s1 s2)); clear; auto.
+  - (*const*)
+    intros. apply prove_errst_spec_ret. refl_case.
+  - (*var*) intros. apply prove_errst_spec_ret. refl_case.
+  - (*if*) intros t t1 t2 t3 Hnode IH1 IH2 IH3.
+    (*By transitivity*)
+    unfold tmap_if_default.
+    repeat (
+    apply prove_errst_spec_bnd_invar with (Q1:=term_wf_pres_cond)(Q2:=term_wf_pres_cond);
+    auto; [| trans_case]; intros).
+    apply errst_spec_err. refl_case.
+  - (*let*)
+    intros t t1 tb Hnode IH1 IH2.
+    apply prove_errst_spec_bnd_invar with (Q1:=term_wf_pres_cond)(Q2:=term_wf_pres_cond);
+    auto; [| trans_case ]. intros e1.
+    (*Now dependent bind*)
+    apply prove_errst_spec_dep_bnd_invar with (Q1:=term_wf_pres_cond)(Q2:=term_wf_pres_cond); 
+    [| | trans_case].
+    + (*t_open_bound*) apply t_open_bound_pres.
+    + (*rest*) intros s2 y Hy. (*bind - first from IH*) 
+      apply prove_errst_spec_bnd_invar with (Q1:=term_wf_pres_cond)(Q2:=term_wf_pres_cond); 
+      auto; [eapply IH2; eauto | | trans_case]. intros.
+      apply errst_spec_err. refl_case.
+  - (*app*) intros t l ts Hnode IH.
+    apply prove_errst_spec_bnd_invar with (Q1:=term_wf_pres_cond)(Q2:=term_wf_pres_cond);
+    auto; [| | trans_case].
+    2: { intros. unfold tmap_app_default. apply prove_errst_spec_ret. refl_case. }
+    (*use loop invariant*)
+    apply prove_errst_spec_list_invar; auto; [| refl_case | trans_case]. 
+    rewrite Forall_map. auto.
+  - (*case*) intros t t1 tbs Hnode IH1 IH2.
+    (*do 1st term*)
+    apply prove_errst_spec_bnd_invar with (Q1:=term_wf_pres_cond)(Q2:=term_wf_pres_cond); auto; [| trans_case].
+    intros s1.
+    (*last part*)
+    apply prove_errst_spec_bnd_invar with (Q1:=term_wf_pres_cond)(Q2:=term_wf_pres_cond);
+    auto; [| | trans_case].
+    2: { intros. unfold tmap_match_default. apply errst_spec_err. refl_case. }
+    (*loop invariant again*)
+    apply prove_errst_spec_list_invar; auto; [| refl_case | trans_case].
+    rewrite Forall_map.
+    (*This one is not quite trivial, need dependent bind*)
+    revert IH2. clear. apply Forall_impl. intros b Hb.
+    apply prove_errst_spec_dep_bnd_invar with (Q1:=term_wf_pres_cond)(Q2:=term_wf_pres_cond); 
+    [| | trans_case]; auto.
+    + apply t_open_branch_pres.
+    + intros s1 b1 Hb1.
+      (*easy bind and return*)
+      apply prove_errst_spec_bnd_invar with (Q1:=term_wf_pres_cond)(Q2:=term_wf_pres_cond); [| | trans_case].
+      * eapply Hb; eauto.
+      * intros. apply prove_errst_spec_ret. refl_case.
+  - (*eps*)
+    intros t b Hnode IH.
+    apply prove_errst_spec_dep_bnd_invar with (Q1:=term_wf_pres_cond)(Q2:=term_wf_pres_cond); 
+    [| | trans_case].
+    + (*t_open_bound*) apply t_open_bound_pres.
+    + (*rest*) intros s2 y Hy. (*bind - first from IH*) 
+      apply prove_errst_spec_bnd_invar with (Q1:=term_wf_pres_cond)(Q2:=term_wf_pres_cond); 
+      auto; [eapply IH; eauto | | trans_case]. intros.
+      apply errst_spec_err. refl_case.
+  - (*quant*) intros t q tq Hnode IH.
+    apply prove_errst_spec_dep_bnd_invar with (Q1:=term_wf_pres_cond)(Q2:=term_wf_pres_cond); 
+    [| | trans_case].
+    + (*t_open_quant1 *) apply t_open_quant1_pres.
+    + intros s1 [[vs1 tr1] t1] Hrun. simpl.
+      specialize (IH _ _ Hrun). simpl in IH. destruct IH as [IH1 IHtr].
+      (*first one*)
+      apply prove_errst_spec_bnd_invar with (Q1:=term_wf_pres_cond)(Q2:=term_wf_pres_cond); [| | trans_case]; auto.
+      intros t2. 
+      (*Do final*)
+      apply prove_errst_spec_bnd_invar with (Q1:=term_wf_pres_cond)(Q2:=term_wf_pres_cond); [| | trans_case].
+      2: { intros x. apply errst_spec_err. refl_case. }
+      (*now do list - doubly nested so trickier*)
+      apply prove_errst_spec_list_invar; auto; [| refl_case | trans_case].
+      rewrite Forall_map.
+      revert IHtr. clear. apply Forall_impl. intros l Hall.
+      apply prove_errst_spec_list_invar; auto; [| refl_case | trans_case].
+      rewrite Forall_map. auto.
+  - (*tbinop*) intros t b t1 t2 Hnode IH1 IH2.
+    repeat (apply prove_errst_spec_bnd_invar with (Q1:=term_wf_pres_cond)(Q2:=term_wf_pres_cond); 
+      [| | trans_case]; auto; intros).
+    apply errst_spec_err. refl_case.
+  - (*tnot*) intros t t1 Hnode IH. 
+    apply prove_errst_spec_bnd_invar with (Q1:=term_wf_pres_cond)(Q2:=term_wf_pres_cond); [| | trans_case]; auto.
+    intros; apply errst_spec_err. refl_case.
+  - (*Ttrue*) intros. apply prove_errst_spec_ret. refl_case.
+  - (*Tfalse*) intros. apply prove_errst_spec_ret. refl_case.
+Qed.
+
+(*Therefore [t_subst_single1] preserves the invariant*)
+Lemma t_subst_single1_pres v t1 t2:
+errst_spec (fun _ : full_st => True) (t_subst_single1 v t1 t2)
+  (fun (s1 : full_st) (_ : term_c) (s2 : full_st) => term_wf_pres_cond s1 s2).
+Proof.
+  unfold t_subst_single1, t_subst1.
+  apply prove_errst_spec_bnd_invar with (Q1:=term_wf_pres_cond)(Q2:=term_wf_pres_cond); 
+  [| | trans_case].
+  1: { apply errst_spec_err. refl_case. }
+  intros _.
+  (*t_make_wf is interesting part*)
+  apply prove_errst_spec_bnd_invar with (Q1:=term_wf_pres_cond)(Q2:=term_wf_pres_cond); 
+  [apply t_make_wf_pres | | trans_case].
+  intros. apply prove_errst_spec_ret. refl_case.
+Qed.
