src/proofs/Gen/InversionLemmas.v
@@ -1,0 +1,161 @@
+Require Import TermFuncs Relations TermTactics.
+From Proofs Require Import Task.
+(*The conditions we have (e.g. evaluation) do not lend themseleves to nice
+  decomposition, so we prove the results here*)
+
+(*TODO: move these*)
+
+(*Inversion Lemmas for eval*)
+Section EvalInv.
+
+(*Const*)
+
+Lemma eval_const_tm {f1 g1 c} 
+  (Hn: t_node_of f1 = TermDefs.Tconst c)
+  (Heval: eval_term f1 = Some g1):
+  exists c1, g1 = Tconst c1 /\ eval_const c = Some c1.
+Proof.
+  destruct_term_node f1. apply option_map_some in Heval. inversion Hn; subst. 
+  destruct Heval as [c1 [Heval Hg1]]; subst. eauto.
+Qed.
+
+Lemma eval_const_fmla {f1 g1 c} 
+  (Hn: t_node_of f1 = TermDefs.Tconst c)
+  (Heval: eval_fmla f1 = Some g1):
+  False.
+Proof.
+  destruct_term_node f1.
+Qed.
+
+(*var*)
+Lemma eval_var_tm {f1 g1 v} 
+  (Hn: t_node_of f1 = TermDefs.Tvar v)
+  (Heval: eval_term f1 = Some g1):
+  g1 = Tvar (eval_vsymbol v).
+Proof.
+  destruct_term_node f1. inversion Heval; subst; auto. inversion Hn; subst; auto.
+Qed.
+
+Lemma eval_var_fmla {f1 g1 v} 
+  (Hn: t_node_of f1 = TermDefs.Tvar v)
+  (Heval: eval_fmla f1 = Some g1):
+  False.
+Proof.
+  destruct_term_node f1.
+Qed.
+
+(*if*)
+
+Lemma eval_if_tm {f1 g1 t1 t2 t3} 
+  (Hn: t_node_of f1 = TermDefs.Tif t1 t2 t3)
+  (Heval: eval_term f1 = Some g1):
+  exists e1 e2 e3, g1 = Tif e1 e2 e3 /\ eval_fmla t1 = Some e1 /\ eval_term t2 = Some e2 /\
+    eval_term t3 = Some e3.
+Proof.
+  destruct_term_node f1.
+  inversion Hn; subst; clear Hn.
+  apply option_bind_some in Heval. destruct Heval as [e1 [He1 Hbind]].
+  apply option_bind_some in Hbind. destruct Hbind as [e2 [He2 Hbind]].
+  apply option_bind_some in Hbind. destruct Hbind as [e3 [He3 Hbind]].
+  inversion Hbind; subst. eauto 10.
+Qed.
+
+Lemma eval_if_fmla {f1 g1 t1 t2 t3} 
+  (Hn: t_node_of f1 = TermDefs.Tif t1 t2 t3)
+  (Heval: eval_fmla f1 = Some g1):
+  exists e1 e2 e3, g1 = Fif e1 e2 e3 /\ eval_fmla t1 = Some e1 /\ eval_fmla t2 = Some e2 /\
+    eval_fmla t3 = Some e3.
+Proof.
+  destruct_term_node f1.
+  inversion Hn; subst; clear Hn.
+  apply option_bind_some in Heval. destruct Heval as [e1 [He1 Hbind]].
+  apply option_bind_some in Hbind. destruct Hbind as [e2 [He2 Hbind]].
+  apply option_bind_some in Hbind. destruct Hbind as [e3 [He3 Hbind]].
+  inversion Hbind; subst. eauto 10.
+Qed.
+
+
+
+(*app - trickier: can become Tfun, Fpred, or Feq*)
+
+Lemma eval_app_tm {f1 g1 l ts}
+  (Hn: t_node_of f1 = TermDefs.Tapp l ts)
+  (Heval: eval_term f1 = Some g1):
+  exists l1 tys' tys1 ts1,
+    g1 = Tfun l1 tys1 ts1 /\ eval_funsym l = Some l1 /\
+      fold_list_option (map term_type ts) = Some tys' /\
+      funpred_ty_list l1 tys' = Some tys1 /\
+      fold_list_option (map eval_term ts) = Some ts1.
+Proof.
+  destruct_term_node f1.
+  inversion Hn; subst; clear Hn.
+  apply option_bind_some in Heval. destruct Heval as [l1 [Hl1 Hbind]]. exists l1.
+  apply option_bind_some in Hbind. destruct Hbind as [ts1 [Hts1 Hbind]].
+  apply option_bind_some in Hbind. destruct Hbind as [tys' [Htsys' Hbind]].
+  apply option_map_some in Hbind. destruct Hbind as [tys1 [Htys1 Hg1]]; subst; eauto 10.
+Qed.
+
+Lemma eval_app_fmla {f1 g1 l ts}
+  (Hn: t_node_of f1 = TermDefs.Tapp l ts)
+  (Heval: eval_fmla f1 = Some g1):
+  (l = ps_equ /\ exists t1 t2 t3 t4 ty1, ts = [t1 ; t2] /\ g1 = Feq ty1 t3 t4 /\
+    eval_term t1 = Some t3 /\ eval_term t2 = Some t4 /\ term_type t1 = Some ty1) \/
+  l <> ps_equ /\
+  exists l1 tys' tys1 ts1,
+    g1 = Fpred l1 tys1 ts1 /\ eval_predsym l = Some l1 /\
+      fold_list_option (map term_type ts) = Some tys' /\
+      funpred_ty_list l1 tys' = Some tys1 /\
+      fold_list_option (map eval_term ts) = Some ts1.
+Proof.
+  destruct_term_node f1.
+  inversion Hn; subst; clear Hn.
+  destruct (lsymbol_eqb l ps_equ) eqn : Heq.
+  - assert (l = ps_equ). apply lsymbol_eqb_eq; auto. subst.
+    left. destruct ts as [| t1 [| t2 [| ? ?]]]; try discriminate.
+    split; auto. exists t1. exists t2. 
+    apply option_bind_some in Heval. destruct Heval as [t3 [Ht3 Hbind]].
+    apply option_bind_some in Hbind. destruct Hbind as [t4 [Ht4 Hbind]].
+    apply option_bind_some in Hbind. destruct Hbind as [ty1 [Hty1 Hbind]].
+    inversion Hbind; subst. eauto 10.
+  - assert (l <> ps_equ).
+    { intro C; subst. assert (Ht: lsymbol_eqb ps_equ ps_equ) by (apply lsymbol_eqb_eq; auto).
+      rewrite Ht in Heq; discriminate.
+    }
+    right. split; auto.
+    apply option_bind_some in Heval. destruct Heval as [l1 [Hl1 Hbind]]. exists l1.
+    apply option_bind_some in Hbind. destruct Hbind as [ts1 [Hts1 Hbind]].
+    apply option_bind_some in Hbind. destruct Hbind as [tys' [Htsys' Hbind]].
+    apply option_map_some in Hbind. destruct Hbind as [tys1 [Htys1 Hg1]]; subst; eauto 10.
+Qed.
+
+(*let*)
+
+Lemma eval_let_tm {f1 g1 t1 tb1} 
+  (Hn: t_node_of f1 = TermDefs.Tlet t1 tb1)
+  (Heval: eval_term f1 = Some g1):
+  exists e1 e2, g1 = Tlet e1 (eval_vsymbol (fst (fst tb1))) e2 /\
+    eval_term t1 = Some e1 /\ eval_term (snd tb1) = Some e2.
+Proof.
+  destruct_term_node f1.
+  inversion Hn; subst; clear Hn.
+  destruct tb1 as [[v1 b1] t2]; simpl.
+  apply option_bind_some in Heval. destruct Heval as [e1 [He1 Hbind]].
+  apply option_bind_some in Hbind. destruct Hbind as [e2 [He2 Hbind]].
+  inversion Hbind; subst. eauto 10.
+Qed.
+
+Lemma eval_let_fmla {f1 g1 t1 tb1} 
+  (Hn: t_node_of f1 = TermDefs.Tlet t1 tb1)
+  (Heval: eval_fmla f1 = Some g1):
+  exists e1 e2, g1 = Flet e1 (eval_vsymbol (fst (fst tb1))) e2 /\
+    eval_term t1 = Some e1 /\ eval_fmla (snd tb1) = Some e2.
+Proof.
+  destruct_term_node f1.
+  inversion Hn; subst; clear Hn.
+  destruct tb1 as [[v1 b1] t2]; simpl.
+  apply option_bind_some in Heval. destruct Heval as [e1 [He1 Hbind]].
+  apply option_bind_some in Hbind. destruct Hbind as [e2 [He2 Hbind]].
+  inversion Hbind; subst. eauto 10.
+Qed.
+
+End EvalInv.
