src/proofs/Gen/TermTactics.v
@@ -1,0 +1,5 @@
+(*TODO: kinda useless for now but need tactics in many places*)
+
+Ltac destruct_term_node t:=
+  let n := fresh "n" in
+  destruct t as [n ? ? ?]; destruct n; try discriminate; simpl in *; subst; simpl in *.
